\section{Interpolation of $L^p$ Spaces}
\subsection{The Lemma of I. I. Hirschman and Hadamard's Three Lines Lemma}

\begin{lemma}[I. I. Hirschman]
	Let $F$ be a holomorphic function in the strip $S := \cbr[0]{z \in \mathbb{C}: 0 < \mathrm{Re}z < 1}$ and continuous on $\overline{S}$, such that for some $0 < A < \infty$ and $0 \leq \tau_0 < \pi$ we have $\log \abs[0]{ F( z )} \leq A e^{\tau_0 \abs[0]{ \Im z}}$ for every $z \in \overline{S}$. Then
	\begin{equation*}
		\abs[0]{ F(z) } \leq \exp\del{ \frac{\sin(\pi x)}{2} \int_{-\infty}^\infty \sbr{ \frac{\log \abs[0]{ F(it + iy)}}{\cosh(\pi t) - \cos(\pi x)} + \frac{\log \abs[0]{ F(1 + it + iy)}}{\cosh(\pi t) + \cos(\pi x)} } \d t}
	\end{equation*}

	\noindent whenever $z := x + iy \in S$.
	\label{lem:hirschman_lemma}
\end{lemma}

\begin{proof}
	We will first prove the case \underline{$y = 0$.} Assume $F$ to be not identically zero (the case where $F$ is identically zero is trivial). Let $h$ be as in lemma (\ref{lem:h}) and let $\zeta := \rho e^{i\theta}$, $0 \leq \rho < 1$. Since $\zeta \in D$, we have $0 < \Re h(\zeta) < 1$ and thus the hypothesis on $F$ and lemma (\ref{lem:upper_bound}) yields
\begin{equation}
	\log \abs[0]{ F(h(\zeta))} \leq Ae^{\frac{\tau_0}{\pi}\abs[0]{ \log \abs[0]{\del[0]{1 + \zeta}/\del[0]{1 - \zeta}}}} \leq Ae^{\tau_0/\pi}\frac{1}{\abs[0]{ \cos(\theta/2) }^{\tau_0/\pi}}\frac{1}{\abs{ \sin(\theta/2) }^{\tau_0/\pi}}
	\label{est:admissible}
\end{equation}

\noindent for $1/(2e - 1) \leq \rho$. Since $0 < \tau_0 < \pi$, inequality (\ref{est:admissible}) asserts, that $\log \abs[0]{ F(h(\zeta))}$ is bounded from above by an integrable function of $\theta$, independently of $\rho \geq 1/(2e - 1)$. Furthermore we have 
	\begin{equation}
		M := \sup\cbr[1]{\log \abs[0]{ F(h(\zeta))} : \zeta \in \overline{B}_{1/\del[0]{2e - 1 }}} < \infty
	\end{equation}

	\noindent since a upper semicontinuous function on a compact space attains its supremum (see lemma \ref{lem:semicom}). Hence
	\begin{equation}
		\log\abs[0]{ F( h( \rho e^{i\theta} ))} \leq \max\cbr[4]{ M,   Ae^{\tau_0/\pi}\frac{1}{\abs[0]{ \cos(\theta/2) }^{\tau_0/\pi}}\frac{1}{\abs[0]{ \sin(\theta/2) }^{\tau_0/\pi}}} =: g( \theta )
		\label{est:log}
	\end{equation}

	\noindent for any $0 \leq \rho < 1$ where $g \in L^1\intcc{-\pi,\pi}$. Let $0 \leq \rho < R < 1$ and $a_1,\dots,a_n$ denote the zeros of $F(h(\zeta))$ for $\abs[0]{ \zeta} < R$ (since $F \circ h$ is holomorphic for $\abs[0]{ \zeta} < 1$ there are indeed only finitely many ones) multiple zeros being repeated. Then for $F(h(\zeta)) \neq 0$ we have by the \emph{Poisson-Jensen formula} (see \cite[208]{ahlfors:complex_analysis:1979})
	\begin{equation}
		\log\abs[0]{ F(h(\zeta))} = - \sum_{k = 1}^n \log\abs[3]{ \frac{R^2 - \overline{a}_k\zeta}{R\del[0]{ \zeta - a_k }}}	+ \frac{1}{2\pi}\int_{-\pi}^\pi \Re \sbr[3]{\frac{R e^{it} + \zeta}{R e^{it} - \zeta}}\log\abs[0]{ F(h(R e^{it}))}\d t
	\end{equation}

	Therefore by
	\begin{equation*}
		\begin{aligned}
			\Re \sbr[3]{\frac{R e^{it} + \zeta}{R e^{it} - \zeta}} &= \Re \sbr[3]{\frac{R^2 - 2i \Im \sbr[0]{ \zeta R e^{-it} } - \abs[0]{ \zeta }^2}{R^2 - 2\Re \sbr[0]{ \zeta R e^{-it} } + \abs[0]{ \zeta }^2}}\\ &= \Re \sbr[3]{\frac{R^2 - 2iR\rho \sin( \theta - t ) - \rho^2 }{R^2 - 2R\rho \cos( \theta - t ) + \rho^2}}\\
			&= \frac{R^2 - \rho^2}{R^2 - 2R\rho \cos( \theta - t ) + \rho^2}
		\end{aligned}
	\end{equation*}

	\noindent and since $\del[0]{ R^2 - \abs[0]{ a_k }^2 }\del[0]{ R^2 - \rho^2 }\geq 0$ for all $k = 1,\dots,n$ implies $\abs[0]{ R^2 - \overline{a}_k\zeta } \geq \abs[0]{ R\del[0]{ \zeta - a_k}}$ the estimate 
	\begin{equation}
		\log\abs[0]{ F(h(\zeta))} \leq \frac{1}{2\pi}\int_{-\pi}^\pi \frac{R^2 - \rho^2}{R^2 - 2R\rho \cos( \theta - t ) + \rho^2}\log\abs[0]{ F(h(R e^{it}))}\d t
	\end{equation}

	\noindent is valid for every $\abs[0]{ \zeta } < R$. By \cite[236]{rudin:rc_analysis:1987} we have
	\begin{equation}
		\frac{R - \rho}{R + \rho} \leq \frac{R^2 - \rho^2}{R^2 - 2R\rho\cos(\theta - \varphi) + \rho^2} \leq \frac{R + \rho}{R - \rho}
		\label{est:poisson}
	\end{equation}
	
	\noindent for $0 \leq \rho < R$. Combining (\ref{est:log}) and (\ref{est:poisson}) yields 
\begin{equation}
	\frac{R^2 - \rho^2}{R^2 - 2R\rho \cos( \theta - t ) + \rho^2}\log\abs[0]{ F(h(\zeta))} \leq \frac{R + \rho}{R - \rho}g( \theta ) =: G( \theta )
\end{equation}

\noindent where $G \in L^1\intcc{-\pi,\pi}$. For $0 < R < 1$ let
\begin{equation*}
	f_R(\varphi) := \frac{R^2 - \rho^2}{R^2 - 2R\rho\cos(\theta - \varphi) + \rho^2}\log\abs[0]{ F(h(Re^{i\varphi}))}
\end{equation*}

\noindent and for $\varphi \notin \cbr[0]{ 0,\pi}$
\begin{equation*}
	f(\varphi) := \frac{1 - \rho^2}{1 - 2\rho\cos(\theta - \varphi) + \rho^2}\log\abs[0]{ F(h(e^{i\varphi}))}
\end{equation*}

Since $\log\abs[0]{ F(h(\zeta))}$ is upper semicontinuous on $\overline{D} \setminus \cbr[0]{ \pm 1}$ by lemma \ref{lem:uppersemcont} we get
\begin{equation*}
	\begin{aligned}
		\limsup_{R \nearrow 1}f_R(\varphi) &= \limsup_{R \nearrow 1} \sbr[3]{ \frac{R^2 - \rho^2}{R^2 - 2R\rho\cos(\theta - \varphi) + \rho^2}\log\abs[0]{ F(h(Re^{i\varphi}))}}\\
		&= \lim_{R \nearrow 1} \frac{R^2 - \rho^2}{R^2 - 2R\rho\cos(\theta - \varphi) + \rho^2}\limsup_{R \nearrow 1} \log\abs[0]{ F(h(Re^{i\varphi}))}\\
		&= \frac{1 - \rho^2}{1 - 2\rho\cos(\theta - \varphi) + \rho^2}\log\abs[0]{ F(h(e^{i\varphi}))} = f(\varphi)
	\end{aligned}
\end{equation*}

\noindent using \cite[363]{bourbaki:general_topology:1995} and proposition \ref{prop:limsup}. The functions $G - f_R$ being non-negative, an application of Fatou's lemma yields
\begin{equation*}
	\int_{-\pi}^\pi \liminf_{R \nearrow 1}\sbr[0]{ G(\varphi) - f_R(\varphi)}\d\varphi \leq \liminf_{R \nearrow 1} \int_{-\pi}^\pi \sbr[0]{ G(\varphi) - f_R(\varphi)}\d\varphi
\end{equation*}

By \cite[354]{bourbaki:general_topology:1995}, we get
\begin{equation*}
	\limsup_{R \nearrow 1} \int_{-\pi}^\pi \sbr[0]{ f_R(\varphi) - G(\varphi)}\d \varphi \leq \int_{-\pi}^\pi \limsup_{R \nearrow 1}\sbr[0]{ f_R(\varphi) - G(\varphi)}\d\varphi
\end{equation*}

\noindent and thus
\begin{equation*}
\begin{aligned}
	\limsup_{R \nearrow 1} \int_{-\pi}^\pi f_R(\varphi) \d\varphi - \int_{-\pi}^\pi G(\varphi)\d\varphi &= \limsup_{R \nearrow 1} \int_{-\pi}^\pi f_R(\varphi) \d\varphi - \lim_{R \nearrow 1}\int_{-\pi}^\pi G(\varphi)\d\varphi\\
	&= \limsup_{R \nearrow 1}\int_{-\pi}^\pi \sbr[0]{ f_R(\varphi) - G(\varphi)}\d\varphi\\
	&\leq \int_{-\pi}^\pi \limsup_{R \nearrow 1} \sbr[0]{f_R(\varphi) - G(\varphi)}\d\varphi\\
	&\leq \int_{-\pi}^\pi \limsup_{R \nearrow 1} f_R(\varphi) \d\varphi - \int_{-\pi}^\pi\lim_{R \nearrow 1} G(\varphi)\d\varphi\\
	&= \int_{-\pi}^\pi \limsup_{R \nearrow 1}f_R(\varphi) \d\varphi - \int_{-\pi}^\pi G(\varphi)\d\varphi
\end{aligned}
\end{equation*}

\noindent by \cite[358]{bourbaki:general_topology:1995}. Hence
\begin{equation*}
	\limsup_{R \nearrow 1} \int_{-\pi}^\pi f_R(\varphi) \d\varphi \leq\int_{-\pi}^\pi \limsup_{R \nearrow 1}f_R(\varphi) \d\varphi
\end{equation*}

\noindent and so 
\begin{equation}
	\log\abs[0]{ F( h( \zeta ) )} \leq \frac{1}{2\pi} \int_{-\pi}^\pi \frac{1 - \rho^2}{1 - 2\rho\cos( \theta - \varphi ) + \rho^2}\log\abs[0]{ F( h( e^{i\varphi}))}\d\varphi	
	\label{eq:limit_case}
\end{equation}

The lemma now follows from (\ref{eq:limit_case}) by a change of variables. By stipulating $x := h( \zeta )$ we obtain 
\begin{multline}
	\zeta = h^{-1}(x) = \frac{e^{\pi i x}- i}{e^{\pi i x} + i} = \frac{\cos(\pi x) + i\sin(\pi x) - i}{\cos(\pi x) + i\sin(\pi x) + i}\\
		= \frac{\cos(\pi x) + i\sin(\pi x) - i}{\cos(\pi x) + i\sin(\pi x) + i}\frac{\cos(\pi x) - i\sin(\pi x) - i}{\cos(\pi x) - i\sin(\pi x) - i}\\
		= -i \frac{\cos(\pi x)}{1 + \sin(\pi x)} = \del[3]{ \frac{\cos(\pi x)}{1 + \sin(\pi x)} }e^{-i\pi/2}
	\label{eq:radius_angle}
\end{multline}

\noindent by
\begin{multline*}
	\del[0]{\cos(\pi x) + i\sin(\pi x) - i}\del[0]{\cos(\pi x) - i\sin(\pi x) - i}\\ = \cos^2(\pi x) - i\sin(\pi x)\cos(\pi x)	
		-i\cos(\pi x) + i\sin(\pi x)\cos(\pi x)\\
	 	+ \sin^2(\pi x) + \sin(\pi x) - i \cos(\pi x) - \sin(\pi x) - 1 = -2i \cos(\pi x)  
\end{multline*}

\noindent and
\begin{multline*}
	\del[0]{ \cos(\pi x) + i\sin(\pi x) + i }\del[0]{ \cos(\pi x) - i\sin(\pi x) - i }\\ = \cos^2(\pi x) - i\sin(\pi x)\cos(\pi x) - i\cos(\pi x) + i\sin(\pi x)\cos(\pi x)\\
	+ \sin^2(\pi x) + \sin(\pi x)+ i \cos(\pi x) + \sin(\pi x) + 1 = 2 + 2\sin(\pi x)
\end{multline*}

	From equality (\ref{eq:radius_angle}) we deduce $\rho = \frac{\cos(\pi x)}{1 + \sin(\pi x)}$, $\theta = -\frac{\pi}{2}$ if $0 < x \leq \frac{1}{2}$ and $\rho = -\frac{\cos(\pi x)}{1 + \sin(\pi x)}$, $\theta = \frac{\pi}{2}$ if $\frac{1}{2} \leq x < 1$. Let $0 < x \leq \frac{1}{2}$. Then we have
\begin{multline*}
	\frac{1 - \rho^2}{1 - 2\rho\cos(\theta - \varphi) + \rho^2} \\= \frac{1 + 2\sin(\pi x) + \sin^2(\pi x) - \cos^2(\pi x)}{1 + 2\sin(\pi x) + \sin^2(\pi x) + 2\cos(\pi x)\sin(\varphi)(1 + \sin(\pi x)) + \cos^2(\pi x)}\\
	= \frac{\sin(\pi x) + \sin^2(\pi x)}{1 + \sin(\pi x) + \cos(\pi x)\sin(\varphi)(1 + \sin(\pi x))}
	= \frac{\sin(\pi x)}{1 + \cos(\pi x)\sin(\varphi)}
\end{multline*}

\noindent and also for $\frac{1}{2} \leq x < 1$. Let $\Phi$ and $\Psi$ be defined as in lemma (\ref{lem:change_of_variables}). We have 
\begin{align*}
	e^{i\Phi(t)} &= h^{-1}(it) = \frac{e^{-\pi t} - i}{e^{-\pi t} + i} \frac{e^{-\pi t} - i}{e^{-\pi t} - i} = \frac{e^{-2\pi t} - 2ie^{-\pi t} - 1}{e^{-2\pi t} + 1} = \frac{e^{-2\pi t} - 1}{e^{-2\pi t} + 1} - \frac{2ie^{-\pi t}}{e^{-2\pi t} + 1}\\ 
	&= \frac{e^{-2\pi t} - 1}{e^{-2\pi t} + 1} - \frac{2i}{e^{-\pi t} + e^{\pi t}} = \frac{1 - e^{2\pi t}}{1 + e^{2\pi t}} - \frac{2i}{e^{-\pi t} + e^{\pi t}} = -\tanh (\pi t) - i \sech(\pi t)
\end{align*}
	
\noindent and thus
\begin{align*}
	\sin( \Phi(t) )\cosh(\pi t) &= \sin( -i\log( -\tanh (\pi t) - i \sech(\pi t) )) \cosh(\pi t)\\
		&= \frac{1}{2i} \sbr[3]{ -\tanh(\pi t) - i\sech(\pi t) + \frac{1}{\tanh(\pi t) + i\sech(\pi t) }}\cosh(\pi t)\\
		&= \frac{1}{2i} \sbr[3]{ \frac{\cosh(\pi t) - \tanh(\pi t) \sinh(\pi t) - 2i\tanh(\pi t) + \sech(\pi t)}{\tanh(\pi t) + i\sech(\pi t)}}\\
		&= \frac{1}{2i} \sbr[3]{ \frac{\cosh^2(\pi t) - \sinh^2(\pi t) - 2i \sinh(\pi t) + 1}{\sinh(\pi t) + i}}\\
		&= \frac{1 - i\sinh(\pi t)}{i\sinh(\pi t) - 1} = -1
\end{align*}

Therefore the transformation formula yields
\begin{equation*}
	\frac{1}{2\pi} \int_{-\pi}^0 \frac{\sin(\pi x)}{1 + \cos(\pi x)\sin(\varphi)} \log \abs[0]{ F(h(e^{i\varphi}))} \d\varphi = \frac{1}{2}\int_{-\infty}^\infty\frac{\sin(\pi x)}{\cosh(\pi t) - \cos(\pi x)} \log\abs[0]{ F(it)} \d t
\end{equation*}
				
\noindent and in a similar manner	
\begin{equation*}
	\frac{1}{2\pi} \int_0^\pi \frac{\sin(\pi x)}{1 + \cos(\pi x)\sin(\varphi)} \log \abs[0]{ F(h(e^{i\varphi}))} \d\varphi = \frac{1}{2}\int_{-\infty}^\infty\frac{\sin(\pi x)}{\cosh(\pi t) + \cos(\pi x)} \log\abs[0]{ F(1 + it) } \d t
\end{equation*}

\noindent holds since
\begin{align*}
		\sin(\Psi(t))\cosh(\pi t) &= \sin( -i\log( -\tanh (\pi t) + i \sech(\pi t) )) \cosh(\pi t)\\
		&= \frac{1}{2i} \sbr[3]{ -\tanh(\pi t) + i\sech(\pi t) - \frac{1}{-\tanh(\pi t) + i\sech(\pi t) }}\cosh(\pi t)\\
		&= \frac{1}{2i} \sbr[3]{ \frac{-\cosh(\pi t) + \tanh(\pi t) \sinh(\pi t) - 2i\tanh(\pi t) - \sech(\pi t)}{-\tanh(\pi t) + i\sech(\pi t)}}\\
		&= \frac{1}{2i} \sbr[3]{ \frac{- \cosh^2(\pi t) + \sinh^2(\pi t) - 2i \sinh(\pi t) - 1}{i - \sinh(\pi t)}}\\
		&= \frac{1 + i\sinh(\pi t)}{1 + i\sinh(\pi t)} = 1
\end{align*}

Thus the case $y = 0$ is prooven.\\
The case \underline{$y \neq 0$.} follows easily from the previous one. Fix $y \neq 0$ and define $G(z) := F(z + iy)$ for $z \in \overline{S}$. Then $G$ is a holomorphic function in $S$ and continuous on $\overline{S}$ as a composition of continuous and holomorphic functions. Moreover, the hypothesis on $F$ yields
	\begin{equation}
		\log \abs[0]{ G(z) } = \log \abs[0]{ F(z + iy) } \leq Ae^{\tau_0 \abs[0]{ \Im z + y}} \leq Ae^{\tau_0 \abs[0]{ \Im z }}e^{\tau_0 \abs[0]{ y }}
	\end{equation}

	for all $z \in \overline{S}$. The previous case yields for $G$ with $A$ replaced by $Ae^{\tau_0\abs[0]{ y }}$
	\begin{equation}
		\abs[0]{ G(x) } \leq \exp\del[3]{ \frac{\sin(\pi x)}{2} \int_{-\infty}^\infty \sbr{ \frac{\log \abs[0]{ G(it)}}{\cosh(\pi t) - \cos(\pi x)} + \frac{\log \abs[0]{ G(1 + it)}}{\cosh(\pi t) + \cos(\pi x)} } \d t}
	\end{equation}

	Now, observing $G(x) = F(x + iy)$, $G(it) = F(it + iy)$ and $G(1 + it) = F(1 + it + iy)$ yields the desired result.
\end{proof}

An almost immediate consequence of the Lemma of I. I. Hirschman \ref{lem:hirschman_lemma} is the so called Hadamard's Three Lines Lemma.

\begin{lemma}[Hadamard's Three Lines Lemma]
	Let $F$ be a holomorphic function in the strip $S := \cbr[0]{ z \in \mathbb{C}: 0 < \Re z < 1}$, continuous and bounded on $\overline{S}$, such that $\abs[0]{F(z)} \leq B_0$ when $\Re z = 0$ and $\abs[0]{F(z)} \leq B_1$ when $\Re z = 1$, for some $0 < B_0,B_1 < \infty$. Then $\abs[0]{F(z)}\leq B_0^{1 - x}B_1^x$ when $\Re z = x$, for any $0 < x < 1$.
	\label{lem:hadamards_three_lines_lemma}
\end{lemma}

\begin{proof}
Let $0 < x < 1$. Then
	\begin{equation*}
		\begin{aligned}
			\frac{\sin( \pi x )}{2} \int_{-\infty}^\infty \frac{1}{\cosh(\pi t ) + \cos( \pi x )} \d t &= \frac{\sin( \pi x )}{2} \int_{-\infty}^\infty \frac{1}{\frac{1}{2}( e^{\pi t} + e^{-\pi t} ) + \cos( \pi x )} \d t\\
			&= \frac{\sin( \pi x )}{\pi} \int_{0}^\infty \frac{1}{s^2 + 2\cos( \pi x )s + 1} \d s\\
			&= \frac{\sin( \pi x )}{\pi} \int_{0}^\infty \frac{1}{( s + \cos( \pi x ) )^2 + \sin^2( \pi x )} \d s\\
			&= \frac{1}{\pi\sin( \pi x )} \int_{0}^\infty \frac{1}{\del{ \frac{s + \cos( \pi x )}{\sin( \pi x )}}^2 + 1} \d s\\
			&= \frac{1}{\pi} \int_{\cot( \pi x )}^\infty \frac{1}{u^2 + 1} \d u\\
			&= \frac{1}{\pi}\sbr{ \frac{\pi}{2} - \arctan( \cot( \pi x )) }\\
			&= x
		\end{aligned}
	\end{equation*}

	\noindent and in the same manner
	\begin{equation*}
		\frac{\sin( \pi x )}{2} \int_{-\infty}^\infty \frac{1}{\cosh( \pi t ) - \cos( \pi x )} \d t = 1 - x	
	\end{equation*}

	Assume that $F$ is holomorphic in $S$, continuous and bounded on $\overline{S}$ with $\abs[0]{F( z )} \leq B_0$ when $\Re z = 0$ and $\abs[0]{F( z )} \leq B_1$ when $\Re z = 1$ for some $0 < B_0, B_1 < \infty$. If $\abs[0]{F( z )} \leq M$ for $0 < M < \infty$, $F$ satisfies the hypothesis with $A := \log( M )$ and $\tau_0 = 0$. Therefore 	
	\begin{equation*}
		\begin{aligned}
			\abs[0]{ F(z) } &\leq \exp\del[3]{ \frac{\sin(\pi x)}{2} \int_{-\infty}^\infty \sbr{ \frac{\log \abs[0]{ F(it + iy)}}{\cosh(\pi t) - \cos(\pi x)} + \frac{\log \abs[0]{ F(1 + it + iy)}}{\cosh(\pi t) + \cos(\pi x)} } \d t}\\
			&\leq \exp\del[3]{ \frac{\sin(\pi x)}{2} \int_{-\infty}^\infty \sbr{ \frac{\log B_0}{\cosh(\pi t) - \cos(\pi x)} + \frac{\log B_1}{\cosh(\pi t) + \cos(\pi x)} } \d t}\\
		&= \exp( x\log B_0 + ( 1 - x)\log B_1 )\\
		&= B_0^xB_1^{1 - x}
		\end{aligned}
	\end{equation*}

	\noindent whenever $z := x + iy \in S$.
\end{proof}

\subsection{The Stein-Weiss Interpolation Theorem for Analytic Families of Operators and the Riesz-Thorin Interpolation Theorem}
\begin{definition}[Analytic family, admissible growth]
	Let $\del{X,\mu}$, $\del{Y,\nu}$ be two $\sigma$-finite measure spaces and $( T_z )_{z \in \overline{S}}$, where $T_z$ is defined $\Sigma_X$ and taking values in the space of all measurable functions on $Y$ such that
	\begin{equation}
		\int_Y \abs[0]{ T_z(\chi_A)\chi_B} \d\nu
	\end{equation}

		\noindent whenever $\mu(A),\nu(B) < \infty$. The family $( T_z )_{z \in \overline{S}}$ is said to be \emph{analytic} if for all $f \in \Sigma_X$, $g \in \Sigma_Y$ we have that

		\begin{equation}
			z \mapsto \int_Y T_z(f)g\d\nu
		\end{equation}

		\noindent is analytic on $S$ and continuous on $\overline{S}$. Further, an analytic family $( T_z )_{z \in \overline{S}}$ is called of \emph{admissible growth}, if there is a constant $\tau_0 \in \intco{0,\pi}$, such that for all $f \in \Sigma_X$, $g \in \Sigma_Y$ a constant $C(f,g)$ exists with

			\begin{equation}
				\log\abs[3]{ \int_Y T_z(f) g \d\nu} \leq C(f,g)e^{\tau_0\abs[0]{ \Im z}}
			\end{equation}

			\noindent for all $z \in \overline{S}$.
	\end{definition}

	\begin{theorem}[Stein-Weiss Interpolation Theorem of Analytic Families of Operators]
		Let $( T_z )_{z \in \overline{S}}$ be an analytic family of admissible growth, $1 \leq p_0,p_1,q_0,q_1 \leq \infty$ and suppose that $M_0$, $M_1$ are positive functions on the real line such that for some $\tau_1 \in \intco{0,\pi}$

			\begin{equation}
				\sup_{-\infty < y <\infty} e^{-\tau_1 \abs[0]{ y }} \log M_0(y) < \infty \qquad \text{and} \qquad \sup_{-\infty < y < \infty} e^{-\tau_1 \abs[0]{ y }} \log M_1(y) < \infty.
				\label{eq:growth_conditions}
			\end{equation}

			Fix $0 < \theta < 1$ and define

			\begin{equation}
				\frac{1}{p} := \frac{1 - \theta}{p_0} + \frac{\theta}{p_1} \qquad \text{and} \qquad \frac{1}{q} := \frac{1 - \theta}{q_0} + \frac{\theta}{q_1}.
			\end{equation}

			Further suppose that for all $f \in \Sigma_X$ and $y \in \mathbb{R}$ we have

			\begin{equation}
				\norm[0]{T_{iy}(f)}_{L^{q_0}} \leq M_0(y)\norm[0]{f}_{L^{p_0}} \qquad \text{and} \qquad \norm[0]{T_{1 + iy}(f)}_{L^{q_1}} \leq M_1(y)\norm[0]{f}_{L^{p_1}}.
			\end{equation}

			Then for all $f \in \Sigma_X$ we have

			\begin{equation*}
				\norm[0]{T_\theta(f)}_{L^q} \leq M(\theta)\norm[0]{f}_{L^p}
			\end{equation*}

			\noindent where for $0 < x < 1$

			\begin{equation*}
				M(x) = \exp\del[3]{ \frac{\sin(\pi x)}{2} \int_{-\infty}^\infty \sbr[3]{ \frac{\log M_0(t)}{\cosh(\pi t) - \cos(\pi x)} + \frac{\log M_1(t)}{\cosh(\pi t) + \cos(\pi x)}} \d t }.
			\end{equation*}
	\end{theorem}

\begin{proof}
	Fix $0 < \theta < 1$ and $f \in \Sigma_X$, $g \in \Sigma_Y$ with $\norm[0]{f}_{L^p} = \norm[0]{g}_{L^{q'}} = 1$. Define $f_z$, $g_z$ as in (\ref{eq:def_fzgz}) and for $z \in \overline{S}$

	\begin{equation*}
		F(z) := \int_Y T_z(f_z)g_z \d\nu	
	\end{equation*}

	Since the family $(T_z)_{z \in \overline{S}}$ is of admissible growth we have that there exist constants $c(\chi_{A_j},\chi_{B_k})$ for any $j = 1,\dots,n$ and $k = 1,\dots,m$ such that 

	\begin{equation*}
		\log\abs[3]{\int_{B_k}T_z\del[0]{\chi_{A_j}}\d \nu} \leq c\del[0]{\chi_{A_j},\chi_{B_k}}e^{\tau_0\abs{\Im z}}
	\end{equation*}

	For shortness we will denote these constants simply by $c(A_j,B_k)$ and get

	\begin{gather*}
		\begin{aligned}
			\log \abs[0]{ F(z) } &= \log \abs[4]{ \sum_{j = 1}^n\sum_{k = 1}^m a^{P(z)}_j b_j^{Q(z)} e^{i\alpha_j} e^{i\beta_k} \int_YT_z(\chi_{A_j})(y)\chi_{B_k}(y)\d\nu(y)}\\
			&\leq \log \sbr[4]{ \sum_{j = 1}^n\sum_{k = 1}^m \max\cbr[0]{1,a_j^{p/p_0 + p/p_1}}\max\cbr[0]{1,b_k^{q'/q'_0 + q'/q'_1}} \abs[3]{\int_{B_k} T_z(\chi_{A_j}) \d\nu}}\\
			&\leq \log\sbr[4]{ \sum_{j = 1}^n\sum_{k = 1}^m \del[0]{ 1 + a_j}^{p/p_0 + p/p_1} \del[0]{1 + b_k}^{q'/q'_0 + q'/q'_1} e^{c(A_j,B_k)e^{\tau_0 \abs[0]{ \Im z}}} }\\
			&\leq  \log\sbr[4]{ \sum_{j = 1}^n\sum_{k = 1}^m e^{\log\del[0]{\del[0]{ 1 + a_j}^{p/p_0 + p/p_1}\del[0]{ 1 + b_k}^{q'/q'_0 + q'/q'_1}} + c(A_j,B_k)e^{\tau_0 \abs[0]{ \Im z}}} }\\
			&\leq \log\del[1]{ mn e^{\sum_{j = 1}^n\sum_{k = 1}^m\log\del[0]{\del[0]{ 1 + a_j}^{p/p_0 + p/p_1} \del[0]{1 + b_k}^{q'/q'_0 + q'/q'_1}} + c(A_j,B_k)e^{\tau_0 \abs[0]{ \Im z}}} }\\
			&= \log(mn) + \sum_{j = 1}^n\sum_{k = 1}^m\log\del[0]{\del[0]{1 + a_j}^{p/p_0 + p/p_1}\del[0]{1 +  b_k}^{q'/q'_0 + q'/q'_1}} + c(A_j,B_k)e^{\tau_0 \abs[0]{ \Im z}}
		\end{aligned}
	\end{gather*}

	\noindent since $\tau_0 \in \intco{0,\pi}$ and thus $e^{\tau_0 \abs[0]{ \Im z}} \geq 1$, $F$ satisfies the hypotheses of the extension of Hadamard's three lines lemma \ref{lem:EHTL} with 

		\begin{equation*}
			A =  \log( mn ) + \sum_{j = 1}^n\sum_{k = 1}^m\del[2]{ \frac{p}{p_0} + \frac{p}{p_1}}\log(1 + a_j) + \del[2]{ \frac{q'}{q'_0} + \frac{q'}{q'_1} } \log( 1 + b_k) + c(A_j,B_k)
	\end{equation*}

	The same calculations as in the proof of the Riesz-Thorin interpolation theorem \ref{thm:Riesz_Thorin} yield for $y \in \mathbb{R}$

	\begin{equation*}
		\norm[0]{ f_{iy}}_{L^{p_0}} = \norm[0]{ f}^{p/p_0}_{L^p} = 1 = \norm[0]{ g}_{L^{q'}}^{q'/q'_0} = \norm[0]{ g_{iy}}_{L^{q_0'}}
	\end{equation*}

	\noindent and

	\begin{equation*}
		\norm[0]{ f_{1 + iy}}_{L^{p_1}} = \norm[0]{ f}^{p/p_1}_{L^p} = 1 = \norm[0]{ g}_{L^{q'}}^{q'/q'_1} = \norm[0]{ g_{1 + iy}}_{L^{q_1'}}
	\end{equation*}

	Further

	\begin{equation*}
		\norm[0]{ F(iy)} \leq \norm[0]{ T_{iy}(f_{iy})}_{L^{q_0}} \norm[0]{ g_{iy}}_{L^{q'_0}} \leq M_0(y) \norm[0]{f_{iy}}_{L^{p_0}}\norm[0]{ g_{iy}}_{L^{q_0'}} = M_0(y)
	\end{equation*}

	\noindent and

	\begin{equation*}
		\norm[0]{ F(1 + iy)} \leq \norm[0]{ T_{1 + iy}(f_{1 + iy})}_{L^{q_1}} \norm[0]{ g_{1 + iy}}_{L^{q'_1}} \leq M_1(y) \norm[0]{f_{1 + iy}}_{L^{p_1}}\norm[0]{ g_{1 + iy}}_{L^{q_1'}} = M_1(y)
	\end{equation*}

	\noindent by H\"older's inequality and the hypotheses on the analytic family $(T_z)_{z \in \overline{S}}$. Therefore the extension of Hadamard's three lines lemma \ref{lem:EHTL} yields

	\begin{equation*}
		\abs[0]{ F(x)} \leq \exp\del[3]{ \frac{\sin(\pi x)}{2} \int_{-\infty}^\infty \sbr[3]{ \frac{\log M_0(t)}{\cosh(\pi t) - \cos(\pi x)} + \frac{\log M_1(t)}{\cosh(\pi t) + \cos(\pi x)}} \d t } = M(x)
	\end{equation*}

	\noindent for every $0 < x < 1$. Furthermore observe that

	\begin{equation*}
		F(\theta) = \int_Y T_\theta(f)g\d\nu
	\end{equation*}

	\noindent and thus by \cite[189]{folland:real_analysis:1999} 

	\begin{gather*}
		\begin{aligned}
			M_q(T_\theta(f)) &= \sup\cbr[3]{ \abs[3]{ \int_Y T_\theta(f) g \d \nu} : g \in \Sigma_Y, \norm[0]{g}_{L^{q'}}}\\
			&= \sup\cbr[0]{ \abs[0]{ F(\theta)} : g \in \Sigma_Y, \norm[0]{ g }_{L^{q'}}}\\
			&\leq M(\theta)
		\end{aligned}
	\end{gather*}

	Since $M(\theta)$ is an absolutely convergent integral (this is immediate by the growth conditions (\ref{eq:growth_conditions})) for any $0 < \theta < 1$, $M_q(T_\theta(f)) < \infty$ and thus $M_q(T_\theta(f)) = \norm[0]{ T_\theta(f)}_{L^q}$. The general statement follows by replacing $f$ with $f/\norm[0]{ f}_{L^p}$ when $\norm[0]{f}_{L^p} \neq 0$. The theorem is trivially true when $\norm[0]{ f}_{L^p} = 0$.
\end{proof}

\begin{theorem}[Riesz-Thorin interpolation theorem]
		Suppose that $\del{X,\mu}$, $\del{Y,\nu}$ are measure spaces and $1 \leq p_0,p_1,q_0,q_1 \leq \infty$. If $q_0 = q_1 = \infty$, suppose also that $\nu$ is semifinite. Let $T$ be a linear operator defined on $\Sigma_X$ and taking values in the set of measurable functions on $Y$, such that for some $0 < M_0,M_1 < \infty$ the estimates 

		\begin{equation}
			\norm[0]{T(f)}_{L^{q_0}} \leq M_0\norm[0]{f}_{L^{p_0}} \quad \text{and} \quad \norm[0]{T(f)}_{L^{q_1}} \leq M_1\norm[0]{f}_{L^{p_1}}
			\label{hyp:Lq0Lq1}
		\end{equation}

		\noindent hold for all $f \in \Sigma_X$. Then for all $0 \leq \theta \leq 1$ we have

		\begin{equation}
			\norm[0]{T(f)}_{L^q} \leq M_0^{1 - \theta}M_1^\theta\norm[0]{f}_{L^p}
			\label{est:boundTf}
		\end{equation}

		\noindent for all $f \in \Sigma_X$, where

		\begin{equation*}
			\frac{1}{p} = \frac{1 - \theta}{p_0} + \frac{\theta}{p_1} \quad \text{and} \quad \frac{1}{q} = \frac{1 - \theta}{q_0} + \frac{\theta}{q_1}.
		\end{equation*}
		\label{thm:riesz_thorin_interpolation_theorem}
\end{theorem}

